working on basic separation logic rules

theorems/machine.v
@@ -1,6 +1,7 @@
 Add LoadPath "/home/blaine/lab/cpdtlib" as Cpdt.
 Set Implicit Arguments. Set Asymmetric Patterns.
 (*Require Import List String Cpdt.CpdtTactics Coq.Program.Wf.*)
+From Coq Require Import Morphisms RelationClasses Setoid.
 Require Import Cpdt.CpdtTactics.
 From stdpp Require Import base options fin gmap.
 (*Import ListNotations.*)
@@ -71,6 +72,15 @@ Module AbstractMachine.
 		apply state_equality; apply map_union_assoc.
 	Qed.
 
+	Theorem state_union_empty_l: forall state: MachineState, union empty state = state.
+	Proof.
+		unfold union, state_union; intros []; simpl; do 2 rewrite map_empty_union; reflexivity.
+	Qed.
+	Theorem state_union_empty_r: forall state: MachineState, union state empty = state.
+	Proof.
+		unfold union, state_union; intros []; simpl; do 2 rewrite map_union_empty; reflexivity.
+	Qed.
+
 	Theorem state_separate_counter_registers_disjoint: forall registers program_counter,
 		state_disjoint (machine_state empty registers) (machine_state program_counter empty).
 	Proof. intros; hnf; simpl; auto with map_disjoint. Qed.
@@ -88,22 +98,28 @@ Module AbstractMachine.
 	Definition state_implies (H1 H2: Assertion): Prop :=
 		forall state, H1 state -> H2 state.
 	Notation "H1 **> H2" := (state_implies H1 H2) (at level 55).
-	Notation "H1 <*> H2" := (state_implies H1 H2 /\ state_implies H2 H1) (at level 60).
+	Definition state_equivalent (H1 H2: Assertion): Prop :=
+		forall state, H1 state <-> H2 state.
+	Notation "H1 <*> H2" := (state_equivalent H1 H2) (at level 60).
 
 	Theorem state_implies_reflexive: forall H, H **> H.
 	Proof. intros; hnf; trivial. Qed.
+	Hint Resolve state_implies_reflexive: core.
 
 	Theorem state_implies_transitive: forall H2 H1 H3,
 		(H1 **> H2) -> (H2 **> H3) -> (H1 **> H3).
 	Proof. intros ??? M1 M2 state H1state; auto. Qed.
+	Hint Resolve state_implies_transitive: core.
 
 	Theorem state_implies_antisymmetric: forall H1 H2,
 		(H1 **> H2) -> (H2 **> H1) -> H1 <*> H2.
 	Proof. intros ?? M1 M2; split; auto. Qed.
+	Hint Resolve state_implies_antisymmetric: core.
 
 	Theorem state_implies_transitive_r: forall H2 H1 H3,
 		(H2 **> H3) -> (H1 **> H2) -> (H1 **> H3).
 	Proof. intros ??? M1 M2; eapply state_implies_transitive; eauto. Qed.
+	Hint Resolve state_implies_transitive_r: core.
 
 	Theorem state_operation_commutative:
 		forall (operation: Assertion -> Assertion -> Assertion),
@@ -111,6 +127,22 @@ Module AbstractMachine.
 			-> (forall H1 H2, operation H1 H2 <*> operation H2 H1).
 	Proof. intros; apply state_implies_antisymmetric; auto. Qed.
 
+	Global Instance state_equivalent_reflexive: Reflexive state_equivalent.
+	Proof. constructor; apply state_implies_reflexive. Qed.
+	Global Instance state_equivalent_symmetric: Symmetric state_equivalent.
+	Proof. hnf; intros ??[]; split; assumption. Qed.
+	Global Instance state_equivalent_transitive: Transitive state_equivalent.
+	Proof. hnf; intros ???[][]; split; eapply state_implies_transitive; eauto. Qed.
+	Global Instance state_equivalence: Equivalence state_equivalent.
+	Proof.
+		constructor; auto using state_equivalent_reflexive, state_equivalent_symmetric,state_equivalent_transitive.
+	Qed.
+	Global Instance subrelation_state_equivalent_implies:
+		subrelation state_equivalent state_implies.
+	Proof. intros ??[]; assumption. Qed.
+
+	Global Instance Proper_state_implies: Proper (state_equivalent ==> state_equivalent ==> flip impl) state_implies.
+	Proof. intros ??[]??[]; hnf; eauto. Qed.
 
 	Definition state_unknown: Assertion := fun state => state = empty.
 	Notation "\[]" := (state_unknown) (at level 0): assertion_scope.
@@ -132,22 +164,22 @@ Module AbstractMachine.
 	Notation "H1 '\*' H2" :=
 		(state_star H1 H2) (at level 41, right associativity): assertion_scope.
 
-	Definition state_exists (X: Type) (P: X -> Assertion): Assertion :=
-		fun state => exists x, P x state.
-	Notation "'\exists' x1 .. xn , H" :=
-		(state_exists (fun x1 => .. (state_exists (fun xn => H)) ..))
+	Definition state_exists (A: Type) (P: A -> Assertion): Assertion :=
+		fun state => exists a, P a state.
+	Notation "'\exists' a1 .. an , H" :=
+		(state_exists (fun a1 => .. (state_exists (fun an => H)) ..))
 		(
-			at level 39, x1 binder, H at level 50, right associativity,
-			format "'[' '\exists' '/ ' x1 .. xn , '/ ' H ']'"
+			at level 39, a1 binder, H at level 50, right associativity,
+			format "'[' '\exists' '/ ' a1 .. an , '/ ' H ']'"
 		): assertion_scope.
 
-	Definition state_forall (X: Type) (P: X -> Assertion): Assertion :=
-		fun state => forall x, P x state.
-	Notation "'\forall' x1 .. xn , H" :=
-		(state_forall (fun x1 => .. (state_forall (fun xn => H)) ..))
+	Definition state_forall (A: Type) (P: A -> Assertion): Assertion :=
+		fun state => forall a, P a state.
+	Notation "'\forall' a1 .. an , H" :=
+		(state_forall (fun a1 => .. (state_forall (fun an => H)) ..))
 		(
-			at level 39, x1 binder, H at level 50, right associativity,
-			format "'[' '\forall' '/ '  x1  ..  xn , '/ '  H ']'"
+			at level 39, a1 binder, H at level 50, right associativity,
+			format "'[' '\forall' '/ '  a1  ..  an , '/ '  H ']'"
 		): assertion_scope.
 
 
@@ -169,33 +201,6 @@ Module AbstractMachine.
 	Theorem state_unknown_inversion: forall state, \[] state -> state = empty.
 	Proof. intros; hnf; auto. Qed.
 
-	(* ### state_pure *)
-	Theorem state_pure_intro: forall P: Prop, P -> \[P] empty.
-	Proof. intros ? P; exists P; hnf; auto. Qed.
-
-	Theorem state_pure_inversion: forall P state, \[P] state -> P /\ state = empty.
-	Proof. intros ?? A; hnf in A; naive_solver. Qed.
-
-	(* ### state_register *)
-	Theorem state_register_intro: forall register value,
-		($register == value) (machine_state empty {[ register := value ]}).
-	Proof. intros; hnf; auto. Qed.
-
-	Theorem state_register_inversion: forall register value state,
-		($register == value) state
-		-> state = (machine_state empty {[ register := value ]}).
-	Proof. intros ??? A; hnf in A; auto. Qed.
-
-	(* ### state_counter *)
-	Theorem state_counter_intro: forall counter,
-		(pc_at counter) (machine_state {[ 0%fin := counter ]} empty).
-	Proof. intros; hnf; auto. Qed.
-
-	Theorem state_counter_inversion: forall counter state,
-		(pc_at counter) state
-		-> state = (machine_state {[ 0%fin := counter ]} empty).
-	Proof. intros ?? A; hnf in A; auto. Qed.
-
 	(* ### state_star *)
 	Theorem state_star_intro: forall (H1 H2: Assertion) s1 s2,
 		H1 s1 -> H2 s2 -> state_disjoint s1 s2
@@ -207,7 +212,6 @@ Module AbstractMachine.
 			H1 s1 /\ H2 s2 /\ state_disjoint s1 s2 /\ state = union s1 s2.
 	Proof. intros ??? A; hnf in A; eauto. Qed.
 
-
 	Theorem state_star_commutative: forall H1 H2,
 		 H1 \* H2 <*> H2 \* H1.
 	Proof.
@@ -217,34 +221,197 @@ Module AbstractMachine.
 		exists s2, s1; repeat split; auto.
 	Qed.
 
-	(*Global Hint Extern 0 (state_union _ _) => (split; assumption): core.*)
-	Hint Rewrite state_union_associative: core.
-
-	Theorem state_star_associative: forall H1 H2 H3,
+	Theorem state_star_associative H1 H2 H3:
 		(H1 \* H2) \* H3 <*> H1 \* (H2 \* H3).
 	Proof.
-intros ???; apply state_implies_antisymmetric.
--
-intros state (state' & h3 & (h1 & h2 & ?&?&?&?)&?& D%symmetry &?); subst state';
-exists h1, (union h2 h3);
-rewrite state_union_associative;
-assert (D' := D);
-apply state_disjoint_union_distributive in D' as [?%symmetry ?%symmetry];
-repeat split; repeat apply state_star_intro; trivial;
-apply state_disjoint_union_distributive; split; trivial.
--
-intros state (h1 & state' &?&(h2 & h3 &?&?&?&?)&D&?); subst state';
-exists (union h1 h2), h3;
-rewrite <-state_union_associative;
-assert (D' := D);
-apply state_disjoint_union_distributive in D' as [];
-repeat split; repeat apply state_star_intro; trivial; symmetry;
-apply state_disjoint_union_distributive; split; symmetry; trivial.
+		apply state_implies_antisymmetric.
+		-
+			intros state (state' & h3 & (h1 & h2 & ?&?&?&?)&?& D%symmetry &?); subst state';
+			exists h1, (union h2 h3);
+			rewrite state_union_associative; assert (D' := D);
+			apply state_disjoint_union_distributive in D' as [?%symmetry ?%symmetry];
+			repeat split; repeat apply state_star_intro; trivial;
+			apply state_disjoint_union_distributive; split; trivial.
+		-
+			intros state (h1 & state' &?&(h2 & h3 &?&?&?&?)&D&?); subst state';
+			exists (union h1 h2), h3;
+			rewrite <-state_union_associative; assert (D' := D);
+			apply state_disjoint_union_distributive in D' as [];
+			repeat split; repeat apply state_star_intro; trivial; symmetry;
+			apply state_disjoint_union_distributive; split; symmetry; trivial.
 	Qed.
 
-	Theorem state_star_empty_l: forall H,
+	Theorem state_star_empty_l H:
 		\[] \* H <*> H.
 	Proof.
+		apply state_implies_antisymmetric; hnf.
+		-
+			intros ? [? (? & ?%state_unknown_inversion & ? & ? & ?)]; subst;
+			rewrite state_union_empty_l; assumption.
+		-
+			intros ?; exists empty, state; repeat split; simpl;
+			try apply state_unknown_intro; try apply map_disjoint_empty_l;
+			try rewrite state_union_empty_l; trivial.
+	Qed.
+
+	Theorem state_star_empty_r H:
+		 H \* \[] <*> H.
+	Proof. rewrite state_star_commutative; apply state_star_empty_l. Qed.
+
+	Theorem state_star_exists A (P: A -> Assertion) H:
+		(\exists a, P a) \* H <*> \exists a, (P a \* H).
+	Proof.
+		apply state_implies_antisymmetric; intros state.
+		- intros (s1 & s2 & (a &?)&?&?&?); exists a, s1, s2; auto.
+		- intros (a & (s1 & s2 &?&?&?&?)); exists s1, s2; split; auto; exists a; trivial.
+	Qed.
+
+	Theorem state_implies_frame_l H2 H1 H1':
+		H1 **> H1' -> (H1 \* H2) **> (H1' \* H2).
+	Proof. intros ?? (s1 & s2 & (?&?&?&?)); exists s1, s2; auto. Qed.
+
+	Theorem state_implies_frame_r H1 H2 H2':
+		H2 **> H2' -> (H1 \* H2) **> (H1 \* H2').
+	Proof. intros ?? (s1 & s2 & (?&?&?&?)); exists s1, s2; auto. Qed.
+
+	(*Theorem state_implies_frame_r' H1 H2 H2':
+		H2 **> H2' -> (H1 \* H2) **> (H1 \* H2').
+	Proof.
+		intros ?; do 2 rewrite (state_star_commutative H1);
+		apply state_implies_frame_l; assumption.
+	Qed.*)
+
+	Theorem state_implies_frame H1 H1' H2 H2':
+		H1 **> H1'
+		-> H2 **> H2'
+		-> (H1 \* H2) **> (H1' \* H2').
+	Proof. intros ??? (s1 & s2 & (?&?&?&?)); exists s1, s2; auto. Qed.
+
+	Theorem state_implies_star_trans_l H1 H2 H3 H4:
+		H1 **> H2
+		-> H2 \* H3 **> H4
+		-> H1 \* H3 **> H4.
+	Proof. intros M1 M2 ? (s1 & s2 & (?&?&?&?)); apply M2; exists s1, s2; auto. Qed.
+
+	Theorem state_implies_star_trans_r H1 H2 H3 H4:
+		H1 **> H2 ->
+		H3 \* H2 **> H4 ->
+		H3 \* H1 **> H4.
+	Proof. intros M1 M2 ? (s1 & s2 & (?&?&?&?)); apply M2; exists s1, s2; auto. Qed.
+
+	(* ### state_pure *)
+	Theorem state_pure_intro: forall P: Prop, P -> \[P] empty.
+	Proof. intros ? P; exists P; hnf; auto. Qed.
+
+	Theorem state_pure_inversion: forall P state, \[P] state -> P /\ state = empty.
+	Proof. intros ?? A; hnf in A; naive_solver. Qed.
+
+	Theorem state_star_pure_l P H state:
+		(\[P] \* H) state <-> P /\ (H state).
+	Proof.
+		unfold state_pure, state_exists; split.
+-
+
+
+hnf.
+rewrite state_star_exists.
+
+
+-
+
+
+		rewrite state_star_exists. rewrite* state_star_empty_l.
+		iff (p&M) (p&M). { split~. } { exists~ p. }
+	Qed.
+
+	Theorem state_star_pure_r: forall P H h,
+		(H \* \[P]) h = (H h /\ P).
+	Proof.
+		intros. rewrite hstar_comm. rewrite state_star_pure_l. apply* prop_ext.
+	Qed.
+
+	Theorem himpl_state_star_pure_r: forall P H H',
+		P ->
+		(H ==> H') ->
+		H ==> (\[P] \* H').
+	Proof. introv HP W. intros h K. rewrite* state_star_pure_l. Qed.
+
+	Theorem state_pure_inv_hempty: forall P h,
+		\[P] h ->
+		P /\ \[] h.
+	Proof.
+		introv M. rewrite <- state_star_pure_l. rewrite~ hstar_hempty_r.
+	Qed.
+
+	Theorem state_pure_intro_hempty: forall P h,
+		\[] h ->
+		P ->
+		\[P] h.
+	Proof.
+		introv M N. rewrite <- (hstar_hempty_l \[P]). rewrite~ state_star_pure_r.
+	Qed.
+
+	Theorem himpl_hempty_state_pure: forall P,
+		P ->
+		\[] ==> \[P].
+	Proof. introv HP. intros h Hh. applys* state_pure_intro_hempty. Qed.
+
+	Theorem himpl_state_star_pure_l: forall P H H',
+		(P -> H ==> H') ->
+		(\[P] \* H) ==> H'.
+	Proof.
+		introv W Hh. rewrite state_star_pure_l in Hh. applys* W.
+	Qed.
+
+	Theorem hempty_eq_state_pure_true :
+		\[] = \[True].
+	Proof.
+		applys himpl_antisym; intros h M.
+		{ applys* state_pure_intro_hempty. }
+		{ forwards*: state_pure_inv_hempty M. }
+	Qed.
+
+	Theorem hfalse_hstar_any: forall H,
+		\[False] \* H = \[False].
+	Proof.
+		intros. applys himpl_antisym; intros h; rewrite state_star_pure_l; intros M.
+		{ false*. } { lets: state_pure_inv_hempty M. false*. }
+	Qed.
+
+	(* ### state_register *)
+	Theorem state_register_intro: forall register value,
+		($register == value) (machine_state empty {[ register := value ]}).
+	Proof. intros; hnf; auto. Qed.
+
+	Theorem state_register_inversion: forall register value state,
+		($register == value) state
+		-> state = (machine_state empty {[ register := value ]}).
+	Proof. intros ??? A; hnf in A; auto. Qed.
+
+	Theorem state_star_register_same register v1 v2:
+		($register == v1) \* ($register == v2) **> \[False].
+	Proof.
+		hnf; intros ? (s1 & s2 & ?%state_register_inversion & ?%state_register_inversion & [] & _);
+		elimtype False; subst; simpl in *;
+		eapply map_disjoint_spec; trivial; apply lookup_singleton.
+	Qed.
+
+	(* ### state_counter *)
+	Theorem state_counter_intro: forall counter,
+		(pc_at counter) (machine_state {[ 0%fin := counter ]} empty).
+	Proof. intros; hnf; auto. Qed.
+
+	Theorem state_counter_inversion: forall counter state,
+		(pc_at counter) state
+		-> state = (machine_state {[ 0%fin := counter ]} empty).
+	Proof. intros ?? A; hnf in A; auto. Qed.
+
+	Theorem state_star_counter v1 v2:
+		(pc_at v1) \* (pc_at v2) **> \[False].
+	Proof.
+		hnf; intros ? (s1 & s2 & ?%state_counter_inversion & ?%state_counter_inversion & [? _] & _);
+		elimtype False; subst; simpl in *;
+		eapply map_disjoint_spec; trivial; apply lookup_singleton.
 	Qed.
 
 	(* ### state_exists *)
@@ -257,18 +424,117 @@ apply state_disjoint_union_distributive; split; symmetry; trivial.
 	Proof. intros ??? A; hnf in A; eauto. Qed.
 
 	(* ### state_forall *)
+	Theorem state_forall_intro: forall A (P: A -> Assertion) state,
+		(forall a, P a state) -> (state_forall P) state.
+	Proof. intros; hnf; assumption. Qed.
 
+	Theorem state_forall_inversion: forall A (P: A -> Assertion) state,
+		(state_forall P) state -> forall a, P a state.
+	Proof. intros; hnf; trivial. Qed.
 
+	(*Theorem state_star_forall H A (P: A -> Assertion):
+		(state_forall P) \* H **> state_forall (P \* H).
+	Proof.
+		intros h M. destruct M as (h1&h2&M1&M2&D&U). intros x. exists~ h1 h2.
+	Qed.*)
 
+	Theorem state_implies_forall_r: forall A (P: A -> Assertion) H,
+		(forall a, H **> P a) -> H **> (state_forall P).
+	Proof. intros ??? M ???; apply M; assumption.  Qed.
 
+	Theorem state_implies_forall_l: forall A a (P: A -> Assertion) H,
+		(P a **> H) -> (state_forall P) **> H.
+	Proof. intros ???? M ??; apply M; trivial. Qed.
 
+	Theorem state_forall_specialize: forall A a (P: A -> Assertion),
+		(state_forall P) **> (P a).
+	Proof. intros; apply (state_implies_forall_l a); auto. Qed.
 
+	(* ### state_wand *)
+	Theorem state_wand_equiv: forall H0 H1 H2,
+		(H0 **> H1 \-* H2) <-> (H1 \* H0 **> H2).
+	Proof.
+		unfold state_wand. iff M.
+		{ rewrite state_star_comm. applys state_implies_state_star_trans_l (rm M).
+			rewrite state_star_state_exists. applys state_implies_state_exists_l. intros H.
+			rewrite (state_star_comm H). rewrite state_star_assoc.
+			rewrite (state_star_comm H H1). applys~ state_implies_state_star_state_pure_l. }
+		{ applys state_implies_state_exists_r H0.
+			rewrite <- (state_star_hempty_r H0) at 1.
+			applys state_implies_frame_r. applys state_implies_hempty_state_pure M. }
+	Qed.
 
+	Theorem state_implies_state_wand_r: forall H1 H2 H3,
+		H2 \* H1 **> H3 ->
+		H1 **> (H2 \-* H3).
+	Proof. introv M. rewrite~ state_wand_equiv. Qed.
 
-	Theorem state_star_exists: forall X (P: X -> Assertion) H,
-		(\exists x, P x) \* H <*> \exists x, (P x \* H).
+	Theorem state_implies_state_wand_r_inv: forall H1 H2 H3,
+		H1 **> (H2 \-* H3) ->
+		H2 \* H1 **> H3.
+	Proof. introv M. rewrite~ <- state_wand_equiv. Qed.
 
-	Theorem state_implies_frame_l: forall H2 H1 H1',
-		H1 **> H1' -> (H1 \* H2) **> (H1' \* H2).
+	Theorem state_wand_cancel: forall H1 H2,
+		H1 \* (H1 \-* H2) **> H2.
+	Proof. intros. applys state_implies_state_wand_r_inv. applys state_implies_refl. Qed.
+
+	Arguments state_wand_cancel: clear implicits.
+
+	Theorem state_implies_hempty_state_wand_same: forall H,
+		\[] **> (H \-* H).
+	Proof. intros. apply state_implies_state_wand_r. rewrite~ state_star_hempty_r. Qed.
+
+	Theorem state_wand_hempty_l: forall H,
+		(\[] \-* H) = H.
+	Proof.
+		intros. applys state_implies_antisym.
+		{ rewrite <- state_star_hempty_l at 1. applys state_wand_cancel. }
+		{ rewrite state_wand_equiv. rewrite~ state_star_hempty_l. }
+	Qed.
+
+	Theorem state_wand_state_pure_l: forall P H,
+		P ->
+		(\[P] \-* H) = H.
+	Proof.
+		introv HP. applys state_implies_antisym.
+		{ lets K: state_wand_cancel \[P] H. applys state_implies_trans K.
+			applys* state_implies_state_star_state_pure_r. }
+		{ rewrite state_wand_equiv. applys* state_implies_state_star_state_pure_l. }
+	Qed.
+
+	Theorem state_wand_curry: forall H1 H2 H3,
+		(H1 \* H2) \-* H3 **> H1 \-* (H2 \-* H3).
+	Proof.
+		intros. apply state_implies_state_wand_r. apply state_implies_state_wand_r.
+		rewrite <- state_star_assoc. rewrite (state_star_comm H1 H2).
+		applys state_wand_cancel.
+	Qed.
+
+	Theorem state_wand_uncurry: forall H1 H2 H3,
+		H1 \-* (H2 \-* H3) **> (H1 \* H2) \-* H3.
+	Proof.
+		intros. rewrite state_wand_equiv. rewrite (state_star_comm H1 H2).
+		rewrite state_star_assoc. applys state_implies_state_star_trans_r.
+		{ applys state_wand_cancel. } { applys state_wand_cancel. }
+	Qed.
+
+	Theorem state_wand_curry_eq: forall H1 H2 H3,
+		(H1 \* H2) \-* H3 = H1 \-* (H2 \-* H3).
+	Proof.
+		intros. applys state_implies_antisym.
+		{ applys state_wand_curry. }
+		{ applys state_wand_uncurry. }
+	Qed.
+
+	Theorem state_wand_inv: forall h1 h2 H1 H2,
+		(H1 \-* H2) h2 ->
+		H1 h1 ->
+		Fmap.disjoint h1 h2 ->
+		H2 (h1 \u h2).
+	Proof.
+		introv M2 M1 D. unfolds state_wand. lets (H0&M3): state_exists_inv M2.
+		lets (h0&h3&P1&P3&D'&U): state_star_inv M3. lets (P4&E3): state_pure_inv P3.
+		subst h2 h3. rewrite union_empty_r in *. applys P4. applys* state_star_intro.
+	Qed.
 
 End AbstractMachine.
